LeanSAT/Reflect/BVExpr/BitBlast.lean
@@ -20,16 +20,19 @@ instance : Inhabited BVBit where
 
 namespace BVExpr
 
--- TODO: Idea for LawfulOperator refactor:
--- TODO: Currently LawfulOperator is only allowed to return Entrypoints. We could instead envision
--- parametrising it over some container that must contain at least an AIG. This would allow the
--- blastVar, blastConst and RefStream APIs to become part of LawfulOperator
-
 namespace bitblast
 
-def blastVar (w : Nat) (aig : AIG BVBit) (idx : Nat) (s : AIG.RefStream aig idx) (a : Nat)
+
+-- TODO: Probably a more general thing that we should put somewhere else
+structure BVVar (width : Nat) where
+  ident : Nat
+
+def blastVar (aig : AIG BVBit) (var : BVVar w) : AIG.RefStreamEntry BVBit w :=
+  go w aig 0 .empty var.ident (by omega)
+where
+  go (w : Nat) (aig : AIG BVBit) (idx : Nat) (s : AIG.RefStream aig idx) (a : Nat)
     (hidx : idx ≤ w)
-    : (aig : AIG BVBit) × AIG.RefStream aig w :=
+    : AIG.RefStreamEntry BVBit w :=
   if hidx:idx < w then
     match haig:aig.mkAtomCached ⟨a, ⟨idx, hidx⟩⟩ with
     | ⟨newAig, bitRef⟩ =>
@@ -40,139 +43,297 @@ def blastVar (w : Nat) (aig : AIG BVBit) (idx : Nat) (s : AIG.RefStream aig idx)
         apply AIG.LawfulOperator.lt_size_of_lt_aig_size (f := AIG.mkAtomCached)
         assumption
       let s := s.pushRef bitRef
-      blastVar w newAig (idx + 1) s a (by omega)
+      go w newAig (idx + 1) s a (by omega)
   else
     have hidx : idx = w := by omega
     ⟨aig, hidx ▸ s⟩
+  termination_by w - idx
+
+theorem blastVar.go_le_size {aig : AIG BVBit} (idx : Nat) (s : AIG.RefStream aig idx) (a : Nat)
+    (hidx : idx ≤ w)
+    : aig.decls.size ≤ (go w aig idx s a hidx).aig.decls.size := by
+  unfold go
+  split
+  . dsimp
+    refine Nat.le_trans ?_ (by apply go_le_size)
+    apply AIG.LawfulOperator.le_size
+  . simp
 termination_by w - idx
 
-theorem blastVar_le_size {aig : AIG BVBit} (idx : Nat) (s : AIG.RefStream aig idx) (a : Nat)
-    (hidx : idx ≤ w)
-    : aig.decls.size ≤ (blastVar w aig idx s a hidx).1.decls.size := sorry
+theorem blastVar_le_size {aig : AIG BVBit} (var : BVVar w)
+    : aig.decls.size ≤ (blastVar aig var).aig.decls.size := by
+  unfold blastVar
+  apply blastVar.go_le_size
 
-theorem blastVar_decl_eq? {aig : AIG BVBit} (i : Nat) (s : AIG.RefStream aig i) (a : Nat)
+theorem blastVar.go_decl_eq? {aig : AIG BVBit} (i : Nat) (s : AIG.RefStream aig i) (a : Nat)
     (hi : i ≤ w)
     : ∀ (idx : Nat) (_hidx : idx < aig.decls.size),
-        (blastVar w aig i s a hi).1.decls[idx]? = aig.decls[idx]? := sorry
-
-theorem blastVar_decl_eq {aig : AIG BVBit} (i : Nat) (s : AIG.RefStream aig i) (a : Nat)
-    (hi : i ≤ w)
-    : ∀ (idx : Nat) (h1) (h2),
-        (blastVar w aig i s a hi).1.decls[idx]'h2 = aig.decls[idx]'h1 := sorry
-
-def blastConst {w : Nat} (aig : AIG BVBit) (idx : Nat) (s : AIG.RefStream aig idx) (val : BitVec w)
-    (hidx : idx ≤ w)
-    : (aig : AIG BVBit) × AIG.RefStream aig w :=
-  if hidx:idx < w then
-    match haig:aig.mkConstCached (val.getLsb idx) with
-    | ⟨newAig, bitRef⟩ =>
-      let s := s.cast <| by
-        intros
-        have : newAig = (aig.mkConstCached (val.getLsb idx)).aig := by rw [haig]
-        rw [this]
-        apply AIG.LawfulOperator.lt_size_of_lt_aig_size (f := AIG.mkConstCached)
+        (go w aig i s a hi).aig.decls[idx]? = aig.decls[idx]? := by
+  intro idx hidx
+  unfold go
+  split
+  . dsimp
+    rw [go_decl_eq?]
+    rw [Array.getElem?_lt, Array.getElem?_lt]
+    . rw [AIG.LawfulOperator.decl_eq (f := AIG.mkAtomCached)]
+      . apply AIG.LawfulOperator.lt_size_of_lt_aig_size (f := AIG.mkAtomCached)
         assumption
-      let s := s.pushRef bitRef
-      blastConst newAig (idx + 1) s val (by omega)
-  else
-    have hidx : idx = w := by omega
-    ⟨aig, hidx ▸ s⟩
+      . assumption
+    . apply AIG.LawfulOperator.lt_size_of_lt_aig_size (f := AIG.mkAtomCached)
+      assumption
+  . simp
+termination_by w - i
+
+theorem blastVar.go_decl_eq {aig : AIG BVBit} (i : Nat) (s : AIG.RefStream aig i) (a : Nat)
+    (hi : i ≤ w)
+    : ∀ (idx : Nat) (h1) (h2), (go w aig i s a hi).aig.decls[idx]'h2 = aig.decls[idx]'h1 := by
+  intro idx h1 h2
+  have := go_decl_eq? i s a hi idx h1
+  rw [Array.getElem?_lt, Array.getElem?_lt] at this
+  injection this
+
+theorem blastVar_decl_eq {aig : AIG BVBit} (var : BVVar w)
+    : ∀ (idx : Nat) (h1) (h2), (blastVar aig var).aig.decls[idx]'h2 = aig.decls[idx]'h1 := by
+  unfold blastVar
+  apply blastVar.go_decl_eq
+
+instance : AIG.LawfulStreamOperator BVBit (fun _ w => BVVar w) blastVar where
+  le_size := by intros; apply blastVar_le_size
+  decl_eq := by intros; apply blastVar_decl_eq
+
+def blastConst (aig : AIG BVBit) (val : BitVec w) : AIG.RefStreamEntry BVBit w :=
+  go aig 0 .empty val (by omega)
+where
+  go {w : Nat} (aig : AIG BVBit) (idx : Nat) (s : AIG.RefStream aig idx) (val : BitVec w)
+      (hidx : idx ≤ w)
+      : AIG.RefStreamEntry BVBit w :=
+    if hidx:idx < w then
+      match haig:aig.mkConstCached (val.getLsb idx) with
+      | ⟨newAig, bitRef⟩ =>
+        let s := s.cast <| by
+          intros
+          have : newAig = (aig.mkConstCached (val.getLsb idx)).aig := by rw [haig]
+          rw [this]
+          apply AIG.LawfulOperator.lt_size_of_lt_aig_size (f := AIG.mkConstCached)
+          assumption
+        let s := s.pushRef bitRef
+        go newAig (idx + 1) s val (by omega)
+    else
+      have hidx : idx = w := by omega
+      ⟨aig, hidx ▸ s⟩
+  termination_by w - idx
+
+theorem blastConst.go_le_size {aig : AIG BVBit} (idx : Nat) (s : AIG.RefStream aig idx) (val : BitVec w)
+    (hidx : idx ≤ w)
+    : aig.decls.size ≤ (go aig idx s val hidx).aig.decls.size := by
+  unfold go
+  split
+  . dsimp
+    refine Nat.le_trans ?_ (by apply go_le_size)
+    apply AIG.LawfulOperator.le_size
+  . simp
 termination_by w - idx
 
-theorem blastConst_le_size {aig : AIG BVBit} (idx : Nat) (s : AIG.RefStream aig idx) (val : BitVec w)
-    (hidx : idx ≤ w)
-    : aig.decls.size ≤ (blastConst aig idx s val hidx).1.decls.size := sorry
+theorem blastConst_le_size {aig : AIG BVBit} (val : BitVec w)
+    : aig.decls.size ≤ (blastConst aig val).aig.decls.size := by
+  unfold blastConst
+  apply blastConst.go_le_size
 
-theorem blastConst_decl_eq? {aig : AIG BVBit} (i : Nat) (s : AIG.RefStream aig i) (val : BitVec w)
+theorem blastConst.go_decl_eq? {aig : AIG BVBit} (i : Nat) (s : AIG.RefStream aig i) (val : BitVec w)
     (hi : i ≤ w)
     : ∀ (idx : Nat) (_hidx : idx < aig.decls.size),
-        (blastConst aig i s val hi).1.decls[idx]? = aig.decls[idx]? := sorry
+        (go aig i s val hi).aig.decls[idx]? = aig.decls[idx]? := by
+  intro idx hidx
+  unfold go
+  split
+  . dsimp
+    rw [blastConst.go_decl_eq?]
+    rw [Array.getElem?_lt, Array.getElem?_lt]
+    . rw [AIG.LawfulOperator.decl_eq (f := AIG.mkConstCached)]
+      . apply AIG.LawfulOperator.lt_size_of_lt_aig_size (f := AIG.mkConstCached)
+        assumption
+      . assumption
+    . apply AIG.LawfulOperator.lt_size_of_lt_aig_size (f := AIG.mkConstCached)
+      assumption
+  . simp
+termination_by w - i
 
-theorem blastConst_decl_eq {aig : AIG BVBit} (i : Nat) (s : AIG.RefStream aig i) (val : BitVec w)
+theorem blastConst.go_decl_eq {aig : AIG BVBit} (i : Nat) (s : AIG.RefStream aig i) (val : BitVec w)
     (hi : i ≤ w)
     : ∀ (idx : Nat) (h1) (h2),
-        (blastConst aig i s val hi).1.decls[idx]'h2 = aig.decls[idx]'h1 := sorry
+        (go aig i s val hi).aig.decls[idx]'h2 = aig.decls[idx]'h1 := by
+  intro idx h1 h2
+  have := blastConst.go_decl_eq? i s val hi idx h1
+  rw [Array.getElem?_lt, Array.getElem?_lt] at this
+  injection this
+
+theorem blastConst_decl_eq {aig : AIG BVBit} (val : BitVec w)
+    : ∀ (idx : Nat) (h1) (h2),
+        (blastConst aig val).aig.decls[idx]'h2 = aig.decls[idx]'h1 := by
+  intros
+  unfold blastConst
+  apply blastConst.go_decl_eq
+
+instance : AIG.LawfulStreamOperator BVBit (fun _ w => BitVec w) blastConst where
+  le_size := by intros; apply blastConst_le_size
+  decl_eq := by intros; apply blastConst_decl_eq
 
 end bitblast
 
-def bitblast (aig : AIG BVBit) (expr : BVExpr w) :
-    (newAig : AIG.ExtendingAIG aig) × AIG.RefStream newAig.val w :=
-  match expr with
-  | .var a =>
-    match haig:bitblast.blastVar w aig 0 .empty a (by omega) with
-    | ⟨newAig, s⟩ =>
-      -- TODO: Think of a way to prettify these theorems
-      ⟨
+def bitblast (aig : AIG BVBit) (expr : BVExpr w) : AIG.RefStreamEntry BVBit w :=
+  go aig expr |>.val
+where
+  go (aig : AIG BVBit) (expr : BVExpr w) : AIG.ExtendingRefStreamEntry aig w :=
+    match expr with
+    | .var a =>
+      match haig:bitblast.blastVar aig ⟨a⟩ with
+      | ⟨newAig, s⟩ =>
+        -- TODO: Think of a way to prettify these theorems
         ⟨
-          newAig,
+          ⟨newAig, s⟩,
           by
-            have : newAig = (bitblast.blastVar w aig 0 .empty a (by omega)).1 :=
-              by simp [haig]
-            rw [this]
-            apply bitblast.blastVar_le_size
-        ⟩,
-        s
-      ⟩
-  | .const val =>
-    match haig:bitblast.blastConst aig 0 .empty val (by omega) with
-    | ⟨newAig, s⟩ =>
-      ⟨
+            have : newAig = (bitblast.blastVar aig ⟨a⟩).aig := by
+              rw [haig]
+            simp only [this]
+            apply AIG.LawfulStreamOperator.le_size
+        ⟩
+    | .const val =>
+      match haig:bitblast.blastConst aig val with
+      | ⟨newAig, s⟩ =>
         ⟨
-          newAig,
+          ⟨newAig, s⟩,
           by
-            have : newAig = (bitblast.blastConst aig 0 .empty val (by omega)).1 := by
+            have : newAig = (bitblast.blastConst aig val).aig := by
               simp [haig]
-            rw [this]
-            apply bitblast.blastConst_le_size
-        ⟩,
-        s
-      ⟩
-  | .bin lhs op rhs =>
-    match op with
-    | .and =>
-      match bitblast aig lhs with
-      | ⟨⟨laig, hlaig⟩, lhs⟩ =>
-        match bitblast laig rhs with
-        | ⟨⟨raig, hraig⟩, rhs⟩ =>
-          let lhs := lhs.cast <| by
-            intro i hi
-            dsimp at hi
-            omega
-          match hfinal:AIG.RefStream.zip raig lhs rhs AIG.mkAndCached with
-          | ⟨finalAig, s⟩ => 
-            ⟨
+            simp only [this]
+            apply AIG.LawfulStreamOperator.le_size
+        ⟩
+    | .bin lhs op rhs =>
+      match op with
+      | .and =>
+        match go aig lhs with
+        | ⟨⟨laig, lhs⟩, hlaig⟩ =>
+          match go laig rhs with
+          | ⟨⟨raig, rhs⟩, hraig⟩ =>
+            let lhs := lhs.cast <| by
+              intro i hi
+              dsimp at hlaig hraig
+              omega
+            match hfinal:AIG.RefStream.zip raig ⟨lhs, rhs, AIG.mkAndCached⟩ with
+            | ⟨finalAig, s⟩ =>
               ⟨
-                finalAig,
+                ⟨finalAig, s⟩,
                 by
-                  have : finalAig = (AIG.RefStream.zip raig lhs rhs AIG.mkAndCached).1 := by
+                  have : finalAig = (AIG.RefStream.zip raig ⟨lhs, rhs, AIG.mkAndCached⟩).aig := by
                     simp [hfinal]
-                  rw [this]
-                  refine Nat.le_trans ?_ (by apply AIG.RefStream.zip_le_size)
+                  simp only [this]
+                  apply AIG.LawfulStreamOperator.le_size_of_le_aig_size
+                  dsimp at hlaig hraig
                   omega
-              ⟩,
-              s
-            ⟩
-  | .un op expr =>
-    match op with
-    | .not =>
-      match bitblast aig expr with
-      | ⟨⟨eaig, heaig⟩, estream⟩ => 
-        match hfinal:estream.map eaig AIG.mkNotCached with
-        | ⟨finalAig, s⟩ => 
-          ⟨
+              ⟩
+    | .un op expr =>
+      match op with
+      | .not =>
+        match go aig expr with
+        | ⟨⟨eaig, estream⟩, heaig⟩ =>
+          match hfinal:AIG.RefStream.map eaig ⟨estream, AIG.mkNotCached⟩ with
+          | ⟨finalAig, s⟩ =>
             ⟨
-              finalAig,
+              ⟨finalAig, s⟩,
               by
-                have : finalAig = (estream.map eaig AIG.mkNotCached).1 := by
+                have : finalAig = (AIG.RefStream.map eaig ⟨estream, AIG.mkNotCached⟩).aig := by
                   simp [hfinal]
-                rw [this]
-                refine Nat.le_trans ?_ (by apply AIG.RefStream.map_le_size)
+                simp only [this]
+                apply AIG.LawfulStreamOperator.le_size_of_le_aig_size
+                dsimp at heaig
                 omega
-            ⟩,
-            s
-          ⟩
+            ⟩
 
--- TODO: LawfulOperator style theorems for bitblast
+theorem bitblast_le_size {aig : AIG BVBit} (expr : BVExpr w)
+    : aig.decls.size ≤ (bitblast aig expr).aig.decls.size := by
+  unfold bitblast
+  exact (bitblast.go aig expr).property
+
+theorem bitblast.go_decl_eq? (aig : AIG BVBit) (expr : BVExpr w)
+    : ∀ (idx : Nat) (_hidx : idx < aig.decls.size),
+        (go aig expr).val.aig.decls[idx]? = aig.decls[idx]? := by
+  intro idx hidx
+  induction expr generalizing aig with
+  | var =>
+    dsimp [go]
+    rw [Array.getElem?_lt, Array.getElem?_lt]
+    rw [AIG.LawfulStreamOperator.decl_eq (f := blastVar)]
+    . apply AIG.LawfulStreamOperator.lt_size_of_lt_aig_size (f := blastVar)
+      assumption
+    . assumption
+  | const =>
+    dsimp [go]
+    rw [Array.getElem?_lt, Array.getElem?_lt]
+    rw [AIG.LawfulStreamOperator.decl_eq (f := blastConst)]
+    . apply AIG.LawfulStreamOperator.lt_size_of_lt_aig_size (f := blastConst)
+      assumption
+    . assumption
+  | bin lhs op rhs lih rih =>
+    cases op with
+    | and =>
+      dsimp [go]
+      rw [Array.getElem?_lt, Array.getElem?_lt]
+      rw [AIG.LawfulStreamOperator.decl_eq]
+      rw [← Array.getElem?_lt, ← Array.getElem?_lt]
+      rw [rih, lih]
+      -- TODO: for some reason my usual omega attempts fail me here
+      . assumption
+      . apply Nat.lt_of_lt_of_le
+        . exact hidx
+        . exact (bitblast.go aig lhs).property
+      . assumption
+      . apply Nat.lt_of_lt_of_le
+        . exact hidx
+        . apply Nat.le_trans
+          . exact (bitblast.go aig lhs).property
+          . exact (go (go aig lhs).1.aig rhs).property
+      . apply AIG.LawfulStreamOperator.lt_size_of_lt_aig_size
+        apply Nat.lt_of_lt_of_le
+        . exact hidx
+        . apply Nat.le_trans
+          . exact (bitblast.go aig lhs).property
+          . exact (go (go aig lhs).1.aig rhs).property
+  | un op expr ih =>
+    cases op with
+    | not =>
+      dsimp [go]
+      rw [Array.getElem?_lt, Array.getElem?_lt]
+      rw [AIG.LawfulStreamOperator.decl_eq]
+      rw [← Array.getElem?_lt, ← Array.getElem?_lt]
+      rw [ih]
+      . assumption
+      . assumption
+      . apply Nat.lt_of_lt_of_le
+        . exact hidx
+        . exact (go aig expr).property
+      . apply AIG.LawfulStreamOperator.lt_size_of_lt_aig_size
+        apply Nat.lt_of_lt_of_le
+        . exact hidx
+        . exact (go aig expr).property
+
+theorem bitblast.go_decl_eq (aig : AIG BVBit) (expr : BVExpr w)
+    : ∀ (idx : Nat) (h1) (h2),
+        (go aig expr).val.aig.decls[idx]'h2 = aig.decls[idx]'h1 := by
+  intro idx h1 h2
+  have := go_decl_eq? aig expr idx h1
+  rw [Array.getElem?_lt, Array.getElem?_lt] at this
+  injection this
+
+theorem bitblast_decl_eq (aig : AIG BVBit) (expr : BVExpr w)
+    : ∀ (idx : Nat) (h1) (h2),
+        (bitblast aig expr).aig.decls[idx]'h2 = aig.decls[idx]'h1 := by
+  intros
+  unfold bitblast
+  apply bitblast.go_decl_eq
+
+instance : AIG.LawfulStreamOperator BVBit (fun _ w => BVExpr w) bitblast where
+  le_size := by intros; apply bitblast_le_size
+  decl_eq := by intros; apply bitblast_decl_eq
 
 end BVExpr
 
@@ -184,25 +345,47 @@ structure ExprPair where
   rhs : BVExpr w
 
 def mkEq (aig : AIG BVBit) (pair : ExprPair) : AIG.Entrypoint BVBit :=
-  let ⟨⟨aig, hlaig⟩, lhsRefs⟩ := pair.lhs.bitblast aig
-  let ⟨⟨aig, hraig⟩, rhsRefs⟩ := pair.rhs.bitblast aig
-  let lhsRefs := lhsRefs.cast <| by
-    intro i hi
-    dsimp at hi
-    omega
-  let ⟨aig, bits⟩ := AIG.RefStream.zip aig lhsRefs rhsRefs AIG.mkBEqCached
-  bits.fold aig AIG.mkAndCached
+  match pair.lhs.bitblast aig with
+  | ⟨laig, lhsRefs⟩ =>
+    match hr:pair.rhs.bitblast laig with
+    | ⟨raig, rhsRefs⟩ =>
+      let lhsRefs := lhsRefs.cast <| by
+        intro i hi
+        have : raig = (pair.rhs.bitblast laig).aig := by
+          simp [hr]
+        rw [this]
+        apply AIG.LawfulStreamOperator.lt_size_of_lt_aig_size (f := BVExpr.bitblast)
+        assumption
+      let ⟨finalAig, bits⟩ := AIG.RefStream.zip raig ⟨lhsRefs, rhsRefs, AIG.mkBEqCached⟩
+      AIG.RefStream.fold finalAig (.mkAnd bits)
 
 theorem mkEq_le_size (aig : AIG BVBit) (target : ExprPair)
     : aig.decls.size ≤ (mkEq aig target).aig.decls.size := by
   unfold mkEq
-  sorry
+  dsimp
+  apply AIG.LawfulOperator.le_size_of_le_aig_size (f := AIG.RefStream.fold)
+  apply AIG.LawfulStreamOperator.le_size_of_le_aig_size (f := AIG.RefStream.zip)
+  apply AIG.LawfulStreamOperator.le_size_of_le_aig_size (f := BVExpr.bitblast)
+  apply AIG.LawfulStreamOperator.le_size (f := BVExpr.bitblast)
 
 theorem mkEq_decl_eq (aig : AIG BVBit) (target : ExprPair) {h : idx < aig.decls.size} :
     have := mkEq_le_size aig target
     (mkEq aig target).aig.decls[idx]'(by omega) = aig.decls[idx]'h := by
   unfold mkEq
-  sorry
+  dsimp
+  rw [AIG.LawfulOperator.decl_eq]
+  rw [AIG.LawfulStreamOperator.decl_eq]
+  rw [AIG.LawfulStreamOperator.decl_eq (f := BVExpr.bitblast)]
+  rw [AIG.LawfulStreamOperator.decl_eq (f := BVExpr.bitblast)]
+  . apply AIG.LawfulStreamOperator.lt_size_of_lt_aig_size (f := BVExpr.bitblast)
+    assumption
+  . apply AIG.LawfulStreamOperator.lt_size_of_lt_aig_size (f := BVExpr.bitblast)
+    apply AIG.LawfulStreamOperator.lt_size_of_lt_aig_size (f := BVExpr.bitblast)
+    assumption
+  . apply AIG.LawfulStreamOperator.lt_size_of_lt_aig_size (f := AIG.RefStream.zip)
+    apply AIG.LawfulStreamOperator.lt_size_of_lt_aig_size (f := BVExpr.bitblast)
+    apply AIG.LawfulStreamOperator.lt_size_of_lt_aig_size (f := BVExpr.bitblast)
+    assumption
 
 instance : AIG.LawfulOperator BVBit (fun _ => ExprPair) mkEq where
   le_size := mkEq_le_size
